#+TITLE: Modulo math
#+LANGUAGE: en
* Shuffling the decks

  After going through the translation, we end up with two constants, the
  deal with increment multiplier $k$, and the cut deck offset $b$.

  Thus, a card \( c \), ends up at position \( p = k \cdot c +
  b~(\mathrm{mod}~m) \).

  Repeating this formula \( n \) times:

  \( p_2 = k (k c + b) + b = k^2 c + k b + b \)

  \( p_3 = k p_2 + b = k (k^2 c + k b + b) + b = k^3c + k^2 b + k b + b
  \)

  \( \cdots \)

  \( p_n = k^n c + k^{n-1} b + k^{n-2} b + \cdots + k^2 b + k b + b \)

  \( p_n = k^n c + b \left( k^{n-1} + \cdots + 1 \right)
  ~(\mathrm{mod}~m)\)

  When we want to find which card that ended up at \( p_n \), we need to
  find the inverse function:

  \( c = \frac{p_n-b \left(k^{n-1} + \cdots + 1\right)}{k^n} \)

  \( = \frac{p_n}{k^n} - \frac{b\left(k^{n-1} + \cdots + 1\right)}{k^n}
  \)

  Multiplying with \( k-1 \) in the last fraction removes the \( \cdots
  \) part and makes things a bit easier.

  \( = \frac{p_n}{k^n} - \frac{b(k^n-1)}{k^n \left(k-1\right)} \)

  \( = \frac{p_n}{k^n} - \frac{b}{k-1} + \frac{b}{k^n(k-1)} \)

  \( = \frac{p_n+\frac{b}{k-1}}{k^n} - \frac{b}{k-1} ~(\textrm{mod}~m)\)

  Since \( a^m = a~(\mathrm{mod}~m) \), we have \( a^{m-2} \cdot a =
  1~(\mathrm{mod}~m) \), and thus \( \frac{1}{a} =
  a^{m-2}~(\mathrm{mod}~m) \).

  Thus:

  \( c = \left(p_n + x\right) \left(k^{m-2}\right)^n - x \) where \( x =
  b \left(k-1\right)^{m-2} \)
